add option for bound vs unbound; regenerate code;

Weidenbach_Book/code/IsaSAT.sml
@@ -80,9 +80,9 @@ fun print_stat (propa, (confl, (dec, (res, lres)))) =
   in
    ()
   end
-fun solver print_modelb print_stats norestart noreduction cnf_name = let
+fun solver print_modelb print_stats norestart noreduction nounbounded cnf_name = let
   val problem = Dimacs_Parser.parse_dimacs_file_map_to_list cnf_name nat_of_lit;
-  val (SAT, stat) = SAT_Solver.isaSAT_code (not norestart, not noreduction) problem ();
+  val (SAT, stat) = SAT_Solver.isaSAT_code (nounbounded, (not norestart, not noreduction)) problem ();
   val _ = (if print_stats then print_stat stat else ());
   val _ =
         (case SAT of
@@ -100,7 +100,8 @@ fun print_help () = (
   println("   conflicts, and decisions. ");
   println("  Use option --model to print a model if one exists.");
   println("  Use option --norestart to deactivate restarts.");
-  println("  Use option --noreduction to DB reduction.")
+  println("  Use option --noreduction to deactivate DB reduction.");
+  println("  Use option --nobounded to force the usage of IntInf.")
 )
 
 fun contains x xs =
@@ -114,6 +115,7 @@ fun process_args [] = print_help()
            (contains "--stat" args)
            (contains "--norestart" args)
            (contains "--noreduction" args)
+           (contains "--nobounded" args)
            (List.last args)
 
 fun main () = let
